unity/models/reschedule.lean
@@ -2,66 +2,117 @@
 import unity.models.nondet
 import unity.refinement
 
-namespace nondet
+universe variable u
 
+def option.cast : ∀ {α β : Type u}, option α → (α = β) → option β
+  | α ._ x rfl := x
+
+def option.cast' : ∀ {α β : Type u}, option α → (β = α) → option β
+  | α ._ x rfl := x
+
+lemma cast_some {α β} (x : α) (P : α = β) : (some x).cast P = some (cast P x) :=
+begin
+  cases P, refl
+end
+
+lemma cast_some' {α β} (x : β) (P : α = β) : (some x).cast' P = some (cast P.symm x) :=
+begin
+  cases P, refl
+end
+
+lemma cast_none : ∀ {α β} (P : α = β), none.cast P = none
+ | α ._ rfl := rfl
+
+lemma cast_none' : ∀ {α β} (P : α = β), none.cast' P = none
+ | α ._ rfl := rfl
+
+lemma cast_cast : ∀ {α β} (P₀ : α = β) (P₁ : β = α) (x : β), cast P₀ (cast P₁ x) = x
+ | α ._ rfl rfl x := rfl
+
+lemma option_cast_cast : ∀ {α β : Type u} (P₀ : α = β) (P₁ : β = α) (x : option β), option.cast(option.cast x P₁) P₀ = x
+ | α ._ rfl rfl (some x) := rfl
+ | α ._ rfl rfl none := rfl
+
+lemma option_cast_cast' : ∀ {α β : Type u} (P₀ P₁ : α = β) (x : option β),
+  option.cast (option.cast' x P₁) P₀ = x
+ | α ._ rfl rfl (some x) := rfl
+ | α ._ rfl rfl none := rfl
+
+namespace nondet
 open predicate
 open unity
 
-universe variable u
+variables {α : Type}
 
-variables {lbl α : Type}
-
-structure evt_ref (mc : @prog α lbl) (ea ec : @event α) : Prop :=
+structure evt_ref (mc : @prog α) (ea ec : @event α) : Prop :=
   (sim : ⟦ ec.step_of ⟧ ⟹ ⟦ ea.step_of ⟧)
   (delay : ea.coarse_sch && ea.fine_sch ↦ ec.coarse_sch in mc)
   (stable : unless mc ec.coarse_sch (~ea.coarse_sch))
   (resched : ea.coarse_sch && ea.fine_sch ↦ ec.fine_sch in mc)
 
-structure refined (ma mc : @prog α lbl) : Prop :=
-  (sim_init : mc^.first ⟹ ma^.first)
-  (sim' : ∀ e, ⟦ mc.step_of e ⟧ ⟹ ⟦ ma.step_of e ⟧)
-  (delay : ∀ e, ma^.coarse_sch_of e && ma^.fine_sch_of e ↦ mc^.coarse_sch_of e in mc)
-  (stable : ∀ e, unless mc (mc^.coarse_sch_of e) (~ma^.coarse_sch_of e))
-  (resched : ∀ e, ma^.coarse_sch_of e && ma^.fine_sch_of e ↦ mc^.fine_sch_of e in mc)
+open temporal
 
-lemma refined.sim {m₀ m₁ : @prog α lbl} (R : refined m₀ m₁)
+structure refined (ma mc : @prog α) : Prop :=
+  (bij : mc.lbl = ma.lbl)
+  (sim_init : mc^.first ⟹ ma^.first)
+  (sim' : ∀ e, ⟦ mc.step_of e ⟧ ⟹ action (ma.step_of (e.cast bij) ))
+  (delay : ∀ e, ma^.coarse_sch_of e && ma^.fine_sch_of e ↦ mc^.coarse_sch_of (e.cast' bij) in mc)
+  (stable : ∀ e, unless mc (mc^.coarse_sch_of e) (~ma^.coarse_sch_of (e.cast bij)))
+  (resched : ∀ e, ma^.coarse_sch_of e && ma^.fine_sch_of e ↦ mc^.fine_sch_of (e.cast' bij) in mc)
+
+lemma refined.sim {m₀ m₁ : @prog α} (R : refined m₀ m₁)
 : ⟦ is_step m₁ ⟧ ⟹ ⟦ is_step m₀ ⟧ :=
 begin
-  simp [is_step_exists_event],
+  simp [is_step_exists_event,R.bij],
   apply p_or_entails_p_or_right,
-  apply p_exists_entails_p_exists, intro e,
-  apply R.sim' (some e),
+  apply p_exists_entails_p_exists' _ _ (λ l, cast R.bij l), intros e τ H,
+  simp,
+  assert H'' : option.cast (some e) (R.bij) = some (cast (R.bij) e),
+  { generalize R.bij P, intro P,
+    rw cast_some },
+  note H' := R.sim' (some e) τ H,
+  rw H'' at H',
+  apply H',
 end
 
-lemma event_refinement {m₀ m₁ : @prog α lbl}
-   (INIT : m₁^.first ⟹ m₀^.first)
-   (EVT : ∀ e, evt_ref m₁ (m₀.event' e) (m₁.event' e))
-: refined m₀ m₁ :=
+lemma event_refinement {ma mc : @prog α}
+   (BIJ : mc.lbl = ma.lbl)
+   (INIT : mc^.first ⟹ ma^.first)
+   (EVT : ∀ e, evt_ref mc (ma.event' e) (mc.event' $ cast BIJ.symm e))
+: refined ma mc :=
 begin
-  apply refined.mk,
+  apply refined.mk BIJ,
   { apply INIT },
   { intro e,
     cases e with e,
-    { simp [step_of_none],
+    { simp [cast_none,step_of_none],
       intro, apply id },
     { unfold prog.step_of prog.event,
-      apply (EVT e).sim } },
+      simp [cast_some],
+      note H := (EVT $ cast BIJ e).sim,
+      simp [cast_cast] at H,
+      apply H } },
   all_goals
     { intro e,
       cases e with e,
-      simp [ prog.coarse_sch_of_none,prog.fine_sch_of_none],
+      simp [ prog.coarse_sch_of_none,prog.fine_sch_of_none,cast_none'],
       try { apply True_leads_to_True },
       try { apply True_unless } },
-  { apply (EVT e).delay },
-  { apply (EVT e).stable },
-  { apply (EVT e).resched },
+  { simp [cast_some'],
+    apply (EVT e).delay },
+  { simp [cast_some],
+    note H := (EVT $ cast BIJ e).stable,
+    simp [cast_cast] at H,
+    apply H },
+  { simp [cast_some'],
+    apply (EVT e).resched },
 end
 
-variables  (m₀ m₁ : @prog α lbl)
+variables  (ma mc : @prog α)
 
 open temporal
 
-theorem soundness : refined m₀ m₁ → unity.refinement.refined m₀ m₁ :=
+theorem soundness : refined ma mc → unity.refinement.refined ma mc :=
 begin
   intros R τ M₁,
   apply nondet.prog.ex.mk,
@@ -71,26 +122,31 @@ begin
     apply R.sim,
     apply M₁.safety },
   { intros e COARSE₀ FINE₀,
-    assert CF_SCH : ([]<>•(prog.coarse_sch_of m₀ e && prog.fine_sch_of m₀ e)) τ,
+    pose e' := e.cast' R.bij,
+    assert CF_SCH : ([]<>•(prog.coarse_sch_of ma e && prog.fine_sch_of ma e)) τ,
     { apply coincidence,
       apply COARSE₀,
       apply FINE₀, },
-    assert COARSE₁ : (<>[]•prog.coarse_sch_of m₁ e) τ,
-    { assert COARSE₂ : ([]<>•prog.coarse_sch_of m₁ e) τ,
+    assert COARSE₁ : (<>[]•prog.coarse_sch_of mc e') τ,
+    { assert COARSE₂ : ([]<>•prog.coarse_sch_of mc e') τ,
       { apply inf_often_of_leads_to (system_sem.leads_to_sem (R.delay e) _ M₁),
         apply CF_SCH },
-      note UNLESS := unless_sem_str _ M₁.safety (R.stable e) COARSE₂,
+      note UNLESS := unless_sem_str _ M₁.safety (R.stable e') COARSE₂,
       cases UNLESS with UNLESS H,
       { apply UNLESS },
-      { assert H' : (~<>[]•prog.coarse_sch_of m₀ e) τ,
-        { rw [not_eventually,not_henceforth,not_init], apply H },
+      { assert H' : (~<>[]•prog.coarse_sch_of ma e) τ,
+        { rw [not_eventually,not_henceforth,not_init],
+          simp [option_cast_cast'] at H,
+          apply H },
         cases H' COARSE₀, } },
-    assert FINE₁ : ([]<>•prog.fine_sch_of m₁ e) τ,
+    assert FINE₁ : ([]<>•prog.fine_sch_of mc e') τ,
     { apply inf_often_of_leads_to (system_sem.leads_to_sem (R.resched _) _ M₁),
       apply CF_SCH, },
     apply hence_map _ _ (M₁.liveness _ COARSE₁ FINE₁),
     apply ex_map,
-    apply R.sim', },
+    note H := R.sim' e',
+    simp [option_cast_cast'] at H,
+    apply H, },
 end
 
 end nondet
